% See instructions in the preamble file
\documentclass[twoside]{article}

\input{preamble/preamble}
\usepackage{hyperref}
\newcommand\pp{\partial}

\begin{document}

%\lecture{**LECTURE-NUMBER**}{**DATE**}{**LECTURER**}{**SCRIBE**}
\lecture{2}{Review Session \#2}{Aliaksandr Zaretski}{Zhikun Lu}
\footnotetext[1]{Visit \url{http://www.luzk.net/misc} for updates.}

\section{Reducible to homogeneous} 
\begin{equation}
    M(x,t)\dd x + N(x,t)\dd t = 0 \quad \text{if} \quad \begin{cases}
        M(\lambda x,\lambda t) = \lambda^k M(x,t)\\
        N(\lambda x,\lambda t) = \lambda^k N(x,t)
    \end{cases}
\end{equation}
\begin{equation}
    \iff \frac{\dd x}{\dd t} = - \frac{N(x,t)}{M(x,t)} = - \frac{(\frac{1}{t})^k N(x,t)}{(\frac{1}{t})^kM(x,t)} = - \frac{N(\frac{x}{t},1)}{M(\frac{x}{t},1)} = f(\frac{x}{t}),
\end{equation}
assuming M and N are homogeneous of order k.

\begin{example}
    $$(t+x)\dd t - (x-t) \dd x = 0 \Longrightarrow \frac{\dd x}{\dd t} = \frac{\frac{x}{t}+1}{\frac{x}{t}-1}$$
    Set $ z = \frac{x}{t}$, then $f(z) = \frac{z+1}{z-1}$.
    \[
    \int \frac{\dd z}{f(z)-z} = \ln |t| + C \Longrightarrow \int \frac{\dd z}{\frac{z+1}{z-1}-z} = \ln |t| + C \Longrightarrow \dots \Longrightarrow \ln |z^2-2z-1| = -2 \ln |t| + C_2
    \]
    \[
    \Longrightarrow |z^2-2z-1| = C_3 |t|^{-2} \Longrightarrow z^2-2z-1 = \frac{C_4}{ t^{2}}
    \]
    \[
    \Longrightarrow (\frac{x}{t})^2 - 2\frac{x}{t} - 1 = \frac{C_4}{ t^{2}} \Longrightarrow x^2 - 2tx - t^2 - C_4 = 0
    \]
    \[
    \Longrightarrow 
    x = t \pm \sqrt{2t^2+C_4}
    \]
\end{example}

\section{Exact ODE}
\begin{equation}
     M(x,t)\dd x + N(x,t)\dd t = 0
\end{equation}
Remember:
\[
    \dd f(x,t) = \frac{\partial f}{\partial x}\dd x + \frac{\partial f}{\partial t}\dd t
\]
If $f = 0$, then $\dd f = 0$. An implication is that
\[
    \frac{\partial M}{\partial t} = \frac{\partial N}{\partial x}
\]
Then $\frac{\partial f}{\partial x} = M(x,t)$ for some $f(x,t) = c$,
\[
    \int \partial f = \int M(x,t) \partial x
\]

\begin{example}
    $(t+x)\dd t - (x-t) \dd x = 0$.

    $\dfrac{\partial M}{\partial t} = 1 = \dfrac{\partial N}{\partial x}$ is satisfied.
    $$\frac{\partial f}{\partial t} = N(x,t) = t+x $$
    $$\int {\partial f}= \int (t+x) \partial t \iff f(x,t) = \frac{t^2}{2} + tx + g(x)$$
    \[
    \Longrightarrow \frac{\partial f}{\partial x} = t + g'(x) = t-x \Longrightarrow g'(x) = -x \Longrightarrow g(x) = - \frac{x^2}{2} + C_1
    \]
    \[
    \Longrightarrow C = f(x,t) =  \frac{t^2}{2} + tx - \frac{x^2}{2} + C_1
    \]
    \[
    \Longrightarrow {x^2} -2tx - {t^2} + C_2 = 0
    \]
    \[
    \Longrightarrow x(t) =  
    \]
\end{example}

\section{Inexact ODE}

\begin{equation}
     M(x,t)\dd x + N(x,t)\dd t = 0
\end{equation}
But $\frac{\partial M}{\partial t} = \frac{\partial N}{\partial x}$ is not satisfied.

Multiplying by $\mu(x,t)$
\begin{equation}
    \Longrightarrow \mu(x,t) M(x,t)\dd x + \mu(x,t) N(x,t)\dd t = 0
\end{equation}
$$\tilde{M}(x,t) = \mu(x,t) M(x,t), \tilde{N}(x,t) = \mu(x,t) N(x,t)$$
Want to find $\mu(x,t)$, such that \[
    \frac{\partial \tilde{M}}{\partial t} = \frac{\partial \tilde{N}}{\partial x}.
\]
%then our previous method could apply.

which implies

\[
    \frac{\pp \mu}{\pp t}M + \mu \frac{\pp M}{\pp t} = \frac{\pp \mu}{\pp x}N + \mu \frac{\pp N}{\pp x}
\]
which is a PDE.

Try $\mu(x)$ or $\mu(t)$

\begin{example}
    \[
    2t \dd x + x \dd t= 0
    \]
    Conjecture $\mu(x)$ (not a function of $t$)
    \[
    \mu(x)2t\dd x + \mu(x)x \dd t = 0 \Longrightarrow \mu(x) = C_1 x
    \]
    Set $C_1 = 1$ w.l.o.g.
    \[
    \Longrightarrow 2tx\dd x + x^2 \dd t = 0
    \]
    then our previous method could apply. (Exercise)
\end{example}

\section{Bernoulli ODE}
\begin{eqnarray}
    &&x' + P(t)x = Q(t)x^n\\
    &\Longrightarrow& x'x^{-n} + P(t)x^{1-n} = Q(t)\\
    &\iff& \frac{1}{1-n} \frac{\dd x^{1-n}}{\dd t} + P(t) x^{1-n} = Q(t)\\
    && \text{Let} \quad z = x^{1-n}\\
    &\Longrightarrow& \frac{1}{1-n} \frac{\dd z}{\dd t} + P(t) z = Q(t)\\
    &\Longrightarrow& \frac{\dd z}{\dd t} + (1-n)P(t) z = (1-n)Q(t)
\end{eqnarray}
which is a first order linear ODE.

\section{First order linear ODE}
$L x(t) = g(t)$, where $L = a_0(t)+a_1(t)\frac{\dd}{\dd t}$
\[
\Longrightarrow a_0(t)x(t)+a_1(t)x'(t) = g(t)
\]
WLOG, set $a_1(t) = 1$, then we get 
\begin{equation}
    x'(t) + a(t)x(t) = g(t) \qquad \text{[C] -- the complete equation}
\end{equation}

\textbf{Variabtion of parameters (constants)/Lagrangian method}

Start with the homogeneous equation [H]
\begin{equation}
    x'(t) + a(t)x(t) = 0 \qquad \text{[H]}
\end{equation}
\begin{eqnarray}
    &\Longrightarrow& \frac{\dd x}{\dd t} = - a(t)x\\
    &&\qquad \vdots \notag\\
    &\Longrightarrow& x(t) = C_3 e^{-\int a(t) \dd t}
\end{eqnarray}
which is the general solution to [H].

Then we look for a particular solution to [C]. Guess \begin{equation}
    x(t) = C(t)e^{-\int a(t) \dd t}
\end{equation}
and substitute into [C], we get
\begin{equation}
    C'(t)e^{-\int a(t) \dd t} + C(t)e^{-\int a(t) \dd t}(-a(t)) + a(t)x(t) = g(t)
\end{equation}
\begin{equation}
    C'(t)e^{-\int a(t) \dd t} = g(t)
\end{equation}
Hence, we have
\begin{equation}
    C'(t) = g(t)e^{\int a(t) \dd t}
\end{equation}
\begin{equation}
    \Longrightarrow \int \dd C = \int g(t)e^{\int a(t) \dd t} \dd t
\end{equation}
\begin{equation}
    C(t) = \int g(t)e^{\int a(t) \dd t} \dd t + C_1
\end{equation}
\begin{equation}
\begin{aligned}
    \Longrightarrow x(t) &= \left (\int g(t)e^{\int a(t) \dd t} \dd t + C_1 \right ) e^{-\int a(t) \dd t}\\
    &= C_1 e^{-\int a(t) \dd t} + e^{-\int a(t) \dd t} \int g(t)e^{\int a(t) \dd t} \dd t
\end{aligned}
\end{equation}
Note that $C_1 e^{-\int a(t) \dd t}$ is a general solution to [H] and $\tilde{C}(t) e^{-\int a(t) \dd t}$ with $\tilde{C}(t) = \int g(t)e^{\int a(t) \dd t} \dd t$ is a particular solution to [C]. Combined together, they form the general solution.
     

















%$$##
\clearpage
\section*{References}
%\beginrefs
%\bibentry{CW87}{\sc D.~Coppersmith} and {\sc S.~Winograd}, 
%``Matrix multiplication via arithmetic progressions,''
%{\it Proceedings of the 19th ACM Symposium on Theory of %Computing},
%1987, pp.~1--6.
%\endrefs

% **** THIS ENDS THE EXAMPLES. DON'T DELETE THE FOLLOWING LINE:

\end{document}

\section{Differential Equations}
\subsection{Basic concepts}
\begin{definition}
    Let $E \in \mathbb{R}$ and $ x \in E \rightarrow \mathbb{R}$ be an unknow function. An ODE of order n is an equation of the from
    $$F(t,x,x',x'', ... , x^{(n)}) = 0$$
    where $F(\cdot)$ is known, real-valued.\\
    This is an implicit equation. We will work with the explicit equations:
    \[
    x^{(n)} = f(t,x,x',x'', ... , x^{(n-1)})
    \]
    $f(\cdot)$ is an known real-valued function.
\end{definition}

\begin{definition}
    Let $E \in \mathbb{R}^k$. An PDE of order n is an equation of the from
    $$F(t,x, \mathrm{D} x,\mathrm{D}^2 x, ... , \mathrm{D}^{n}x) = 0$$
    where $F(\cdot)$ is known, real-valued.
\end{definition}

This is an implicit equation. We will work with the explicit equations:
\[
x^{(n)} = f(t,x,x',x'', ... , x^{(n-1)})
\]
$f(\cdot)$ is an known real-valued function.

\begin{example} (ODE)
    \[
    [x'''(t)]^4 + e^{- \xi t} x''(t) + x(t) = \tan t
    \]
    Here, the order is 3, the degree is 4., exogenous variable: $t$, endogenous variable: $x$.
\end{example}

\begin{theorem}
    Let $E \in \mathbb{R}^2$, and $f: E \rightarrow \mathbb{R}$. If $f$ is continuously differentiable ($C^1$) at $(t_0, x_0) \in E$, then $\exists \epsilon > 0$ and a unique $C^1$ function $t \mapsto x(t)$, such that 
    $$x'(t) = f(t,x(t)), \forall t \in (t_0- \epsilon, t_0 + \epsilon),$$ and also $x(t_0) = x_0$
\end{theorem}

\begin{remark} 
    A \underline{general solution} to an ODE is a set of all solutions.
    A \underline{particular solutions} is a solution that satisfies \underline{initial conditions}.
\end{remark}

The number of initial conditions must be equal to the order of an ODE. For example, if you solve 
$$
x^{(n)}(t) = f(t, x', ..., x^{(n-1)})
$$
provide $x(t_0),x'(t_0), ..., x^{(n-1)}(t_0).$

\begin{definition}
    An ODE is linear if it takes the form $\mathrm{L}x(t) = g(t)$, where g is a known real-valued function, L is the linear differential operator,
    \[
    \mathrm{L} = a_0(t) + a_1(t)\frac{\dd }{\dd t}+ ... + a_n(t)\frac{\dd^n }{\dd t^n}.
    \]
    Then $$\mathrm{L}x(t) = a_0(t) x(t) + a_1(t)\frac{\dd x(t)}{\dd t}+ ... + a_n(t)\frac{\dd^n x(t)}{\dd t^n} = g(t)$$
\end{definition}

\begin{definition}
    An ODE is nonlinear if it is not linear.
\end{definition}

\subsection{Some common types of ODE}
\subsubsection{Separable ODEs}
\begin{equation}
    \begin{aligned}
        x'(t) = f(x)g(t) &\Longrightarrow \frac{\dd x}{\dd t} = f(x)g(t) \Longrightarrow
        \frac{\dd x}{f(x)}  = g(t) \dd t\\
        &\Longrightarrow \int \frac{\dd x}{f(x)}  = \int g(t) \dd t
    \end{aligned}
\end{equation}

\begin{example}
    \begin{equation}
    \begin{aligned}
        \frac{\dd x}{\dd t} = \frac{x}{t} \iff \int \frac{\dd x}{x} = \int \frac{ \dd t}{t}
        \Longrightarrow 
        \ln |x| = \ln |t| + C_1
        &\Longrightarrow 
        |x| = |t| e^{C_1} \equiv C_2 |t|\\
        &\Longrightarrow x = C_3 t
    \end{aligned}
    \end{equation}
    Suppose $x(1) = 5$, then $|x| = C_2 |t| \Longrightarrow x(t) = 5t$.
\end{example}

\subsubsection{Reducible to separable} 
Suppose we have
\[
x'(t) = f(a x + b t + c)
\]
Let $z = a x + b t + c$, then $z'(t) = a x'(t)+b = f(z) + b$, then $\frac{\dd z}{a f(z) + b} = \dd t$,
\[
    \int \frac{\dd z}{a f(z) + b} = \int \dd t = t + C_1
    \Longrightarrow \text{solve for } z(t) \Longrightarrow \text{solve for } x(t)
\]

\begin{example}
    Let $a = -1, b=1, c= 0$,
    \[
    \frac{\dd x}{\dd t} = \frac{1}{t-x} + 1
    \]
    The left hand side seems not separable. Let $z = t-x$, so $f(z) = \frac{1}{z}+1$. Then 
    \[
    \int \frac{\dd z}{-\frac{1}{z}-1+1} = t + C_1
    \iff \int z \dd z = -t - C_1 \Longrightarrow \frac{z^2}{2} = -t + C_2 \iff {z^2} = -2t + C_3
    \]
    \begin{equation}
    x(t) = t \pm \sqrt{-2t + C_3} \quad \text{- general solution}
    \end{equation}
    With initial condition $x(0) = 5$, then $5 = \pm \sqrt{C_3} \Longrightarrow C_3 = 25$. Hence
    \begin{equation}
        x(t) = t + \sqrt{-2t + 25} \quad \text{- particular solution}
    \end{equation}
\end{example}

\subsection{Homogeneous ODEs}
Homogeneous ODEs have the following form
\[
\frac{\dd x}{\dd t} = f(\frac{x}{t})
\]
Let $z = \dfrac{x}{t} \Longrightarrow x(t) = t z(t), x'(t) = z(t) + t z'(t) $. 
Hence, the original ODE can be transformed into
\begin{equation}
    z(t) + t z'(t) = f(z) \Longrightarrow \frac{\dd z}{f(z) - z} = \frac{\dd t}{t}
\end{equation}
\begin{equation}
    \int \frac{\dd z}{f(z) - z} = \ln |t| + C
\end{equation}

\begin{example}
    $\frac{\dd x}{\dd t} = \tan(\frac{x}{t}) + \frac{x}{t}$. So $ f(z) = \tan z + z $. Hence
    \begin{equation}
        \int \frac{\dd z}{\tan z} = \ln |t| + C \Longrightarrow \ln | \sin z| = \ln |t| + C \iff |\sin z | = C_1 |t| \iff z(t) = \arcsin (C_2 t)
    \end{equation}
    \begin{equation}
        \Longrightarrow \frac{x(t)}{t} = \arcsin (C_2 t) \Longrightarrow x(t) = t \arcsin (C_2 t) \quad \text{-\quad general solution}
    \end{equation}
    Now suppose $x(t_0) = x_0$, ..., 
    \begin{equation}
        \Longrightarrow x(t) = t \arcsin (\frac{t}{t_0}\sin(\frac{x_0}{t_0}))
    \end{equation}
\end{example}




